\documentclass{article}
\usepackage[utf8]{inputenc}

\title{Test 1 Corrections}
\author{Matthew Zhang}
\date{October 2018}

\begin{document}

\maketitle

\section{Problem 4}
Begin with an expression of the cosine angle addition identity
\\
$$cos(2x+8x)=cos(2x)cos(8x)-sin(2x)sin(8x)$$
\\
One could notice that through clever use of the cosine angle subtraction identity
($cos(2x-8x)=cos(2x)cos(8x)+sin(2x)sin(8x)$)
the cosine terms on the right hand side could be eliminated, as follows:
$$cos(2x+8x)-cos(2x-8x)=cos(2x)cos(8x)-sin(2x)sin(8x)-[cos(2x)cos(8x)+sin(2x)sin(8x)]$$
Simplifying yields
$$cos(2x+8x)-cos(2x-8x)=-2sin(2x)sin(8x)$$
$$\frac{-cos(2x+8x)+cos(2x-8x)}{2}=sin(2x)sin(8x)$$
\clearpage
\section{Problem 5}
$$\int sin^{11}x\; cos^6x\;dx$$
$$\int sinx\; (1-cos^2x)^5\; cos^6x\;dx$$

$$u=cosx$$
$$du=-sinx\;dx$$

$$-\int (1-u^2)^5\; u^6\;du$$
$$-\int (1-5u^2+10u^4-10u^6+5u^8-u^{10})\; u^6\;du$$
$$-\int (u^6-5u^8+10u^{10}-10u^{12}+5u^{14}-u^{16})\; du$$
$$-(\frac{u^7}{7}-\frac{5u^9}{9}+\frac{10u^{11}}{11}-\frac{10u^{13}}{13}+\frac{u^{15}}{3}-\frac{u^{17}}{17})+C$$
$$-\frac{u^7}{7}+\frac{5u^9}{9}-\frac{10u^{11}}{11}+\frac{10u^{13}}{13}-\frac{u^{15}}{3}+\frac{u^{17}}{17}+C$$

$$-\frac{cos^7x}{7}+\frac{5cos^9x}{9}-\frac{10cos^{11}x}{11}+\frac{10cos^{13}x}{13}-\frac{cos^{15}x}{3}+\frac{cos^{17}x}{17}+C$$
\clearpage
\section{Problem 7}
$$\frac{a}{2x-3}+\frac{b}{x+2}=\frac{3x-5}{(2x-3)(x+2)}$$

$$ax+2a+2bx-3b=3x-5$$
\center{Substitute -2 for x}
$$-7b=-5-6$$
$$b=\frac{11}{7}$$
\center{Substitute $\frac{3}{2}$ for x}
$$\frac{7}{2}a=\frac{9}{2}-5$$
$$\frac{7}{2}a=-\frac{1}{2}$$
$$a=-\frac{1}{7}$$
Plug in and integrate
$$\int \frac{-1}{7(2x-3)}dx+\int \frac{11}{7(x+2)}dx$$
$$\frac{-ln|2x-3|}{14}+ \frac{-11ln|x+2|}{7}+C$$


\end{document}
